src/spec/properties/TLS13.ConnectionState.ProtectedWireServerFlight.fsti
@@ -12,6 +12,80 @@ module WFL = TLS13.Spec.WireFormatLemmas
 
 open TLS13.ConnectionState.ProtectedWireBase
 
+val lemma_single_message_sender_after_server_write_client_read_install_normalizes_received_head
+  (server:CS.connection_model)
+  (client:CS.connection_model)
+  (server_material:CS.traffic_key_material)
+  (client_material:CS.traffic_key_material)
+  (sent_msg:M.handshake_msg)
+  (received_msg:M.handshake_msg)
+  (client_head:CS.conn_event)
+  (server_rest:list CS.conn_event)
+  (client_rest:list CS.conn_event)
+  (server_raw_sent:B.bytes)
+  (server_raw_received:B.bytes)
+  (client_raw_sent:B.bytes)
+  (client_raw_received:B.bytes)
+  (server_final:CS.connection_model)
+  (client_final:CS.connection_model)
+  : Lemma
+      (requires
+        (match
+          server.CS.model_handshake.CS.hs_keys.CS.ks_handshake_secret,
+          client.CS.model_handshake.CS.hs_keys.CS.ks_handshake_secret
+        with
+        | Some server_secret, Some client_secret ->
+          Seq.equal server_secret client_secret
+        | _, _ ->
+          False) /\
+        Seq.equal
+          server.CS.model_handshake.CS.hs_transcript
+          client.CS.model_handshake.CS.hs_transcript /\
+        CS.protected_handshake_buffer_empty client /\
+        Seq.equal server_raw_sent client_raw_received /\
+        protected_handshake_wire_round_trip_message sent_msg /\
+        (match client_head with
+         | CS.ConnNetworkEvent directed ->
+           directed.CL.message_direction == CL.Received /\
+           directed.CL.message_value == M.TlsHandshake received_msg
+         | CS.ConnProtectedHandshake step ->
+           step.CS.protected_handshake_message == received_msg
+         | CS.ConnLocalEvent _ ->
+           False) /\
+        TLS13.Spec.StateMachine.Replay.conn_events_sent_seal_replay
+          server
+          (CS.ConnLocalEvent
+            (CS.LocalInstallTrafficKeysForRole {
+              CS.install_role = CS.ServerEndpoint;
+              CS.install_payload = {
+                CS.install_epoch = CS.TrafficHandshake;
+                CS.install_direction = CS.TrafficWrite;
+                CS.install_material = server_material;
+              };
+            }) :: CS.ConnNetworkEvent {
+              CL.message_direction = CL.Sent;
+              CL.message_value = M.TlsHandshake sent_msg;
+            } :: server_rest)
+          server_raw_sent
+          server_raw_received
+          server_final /\
+        TLS13.Spec.StateMachine.Replay.conn_events_received_decode_replay
+          client
+          (CS.ConnLocalEvent
+            (CS.LocalInstallTrafficKeys {
+              CS.install_epoch = CS.TrafficHandshake;
+              CS.install_direction = CS.TrafficRead;
+              CS.install_material = client_material;
+            }) :: client_head :: client_rest)
+          client_raw_sent
+          client_raw_received
+          client_final)
+      (ensures
+        client_head == CS.ConnNetworkEvent {
+          CL.message_direction = CL.Received;
+          CL.message_value = M.TlsHandshake received_msg;
+        })
+
 val lemma_protected_handshake_event_projection_pair_after_server_write_client_read_install_heads_with_tails
   (server:CS.connection_model)
   (client:CS.connection_model)
